feat: overflowing_mul

backends/lean/Aeneas/Std/Scalar/OverflowingOps.lean
@@ -164,5 +164,85 @@ theorem core.num.«%S».overflowing_sub_eq (x y : «%S») :
   else  z.fst.val = x.val - y.val ∧ z.snd = false
   := UScalar.overflowing_sub_eq x y
 
+def UScalar.overflowing_mul {ty} (x y : UScalar ty) : UScalar ty × Bool :=
+  (⟨ x.bv * y.bv ⟩, 2^ty.numBits ≤ x.val * y.val)
+
+def IScalar.overflowing_mul {ty} (x y : IScalar ty) : IScalar ty × Bool :=
+  (⟨ x.bv * y.bv ⟩,
+     ¬ (-2^(ty.numBits -1) ≤ x.val * y.val ∧ x.val * y.val < 2^(ty.numBits-1)))
+
+/- [core::num::{u8}::overflowing_mul] -/
+uscalar def core.num.«%S».overflowing_mul := @UScalar.overflowing_mul .«%S»
+
+/- [core::num::{i8}::overflowing_mul] -/
+iscalar def core.num.«%S».overflowing_mul := @IScalar.overflowing_mul .«%S»
+
+theorem UScalar.overflowing_mul_eq {ty} (x y : UScalar ty) :
+  let z := overflowing_mul x y
+  if x.val * y.val > UScalar.max ty then
+    z.fst.val = (x.val * y.val) % UScalar.size ty ∧
+    z.snd = true
+  else
+    z.fst.val = x.val * y.val ∧
+    z.snd = false
+  := by
+  simp [overflowing_mul]
+  simp only [val, BitVec.toNat_mul, max]
+  split <;> rename_i hLt
+  · split_conjs
+    · simp [size]
+    · omega
+  · split_conjs
+    · apply Nat.mod_eq_of_lt
+      grind
+    · grind
+
+uscalar @[step_pure overflowing_mul x y]
+theorem core.num.«%S».overflowing_mul_eq (x y : «%S») :
+  let z := overflowing_mul x y
+  if x.val * y.val > UScalar.max .«%S» then z.fst.val = (x.val * y.val) % UScalar.size .«%S» ∧ z.snd = true
+  else z.fst.val = x.val * y.val ∧ z.snd = false
+  := UScalar.overflowing_mul_eq x y
+
+theorem UScalar.overflowing_mul_comm {ty} (x y : UScalar ty) :
+  overflowing_mul x y = overflowing_mul y x := by
+  simp [overflowing_mul, Nat.mul_comm]
+  exact BitVec.mul_comm x.bv y.bv
+
+theorem IScalar.overflowing_mul_comm {ty} (x y : IScalar ty) :
+  overflowing_mul x y = overflowing_mul y x := by
+  simp [IScalar.overflowing_mul, Int.mul_comm]
+  exact BitVec.mul_comm x.bv y.bv
+
+uscalar
+theorem core.num.«%S».overflowing_mul_comm (x y : «%S») :
+  overflowing_mul x y = overflowing_mul y x := UScalar.overflowing_mul_comm x y
+
+iscalar
+theorem core.num.«%S».overflowing_mul_comm (x y : «%S») :
+  overflowing_mul x y = overflowing_mul y x := IScalar.overflowing_mul_comm x y
+
+theorem UScalar.overflowing_mul_assoc {ty} (x y z : UScalar ty) :
+  (overflowing_mul (overflowing_mul x y).1 z).1 = (overflowing_mul x (overflowing_mul y z).1).1 := by
+  simp [overflowing_mul]
+  exact BitVec.mul_assoc x.bv y.bv z.bv
+
+theorem IScalar.overflowing_mul_assoc {ty} (x y z : IScalar ty) :
+  (overflowing_mul (overflowing_mul x y).1 z).1 = (overflowing_mul x (overflowing_mul y z).1).1 := by
+  simp [overflowing_mul]
+  exact BitVec.mul_assoc x.bv y.bv z.bv
+
+uscalar
+theorem core.num.«%S».overflowing_mul_assoc (x y z : «%S») :
+  (overflowing_mul (overflowing_mul x y).1 z).1 = (overflowing_mul x (overflowing_mul y z).1).1 :=
+  UScalar.overflowing_mul_assoc x y z
+
+iscalar
+theorem core.num.«%S».overflowing_mul_assoc (x y z : «%S») :
+  (overflowing_mul (overflowing_mul x y).1 z).1 = (overflowing_mul x (overflowing_mul y z).1).1 :=
+  IScalar.overflowing_mul_assoc x y z
+
+
+
 
 end Aeneas.Std
